
## 7.1 Basic Notions

example CFG 

Σ1= {a,b}   <- terminals
V = {S,A,B}   <- vars/nonterminals 

_substitution rules_
~~~
S-> A
S-> B
A-> aA
A->ε
B->bBa
B->ε
~~~

A derivation:
S-> A           rule 1
   -> aAb      rule 3
   -> aaAbb  rule 3
   -> aaaAbbb  rule 3
   -> aaabbb rule 4

(continue deriving until no more variables)


Def: 
the lang of a grammar G is the set of all strings that can be derived


ex: 
S - > A|B  (pipe operater is short for alternation btw so its S -> A   S-> B)
A - > aAb | ε
B - > bBa | ε

Lang: 
{a^n b^n: n>= 0} u 
{b^n a^n: n>= 0}

Def A grammar is a tuple 
(V,Σ,R,S)
where 
V = set of vars (finite nonempty)
Σ = set of terminals 
R = set of rules 
S = start variable 

## 7.2 reading CFG's 
the : n or :n,m >= x means where n or n and m are >= x
ex 
S -> AA
~~A -> A~~
- (doesnt terminate, nonsense grammar. we get ∅. replacing a var with itself is implicit and doesnt change anything we can cross it out) 

ex 
S -> abS|a
- (ab)* a

ex
S-> aSb | ε
 - a^n b^n :n >= 0

ex 
S-> aSa|B
B-> bB|ε
 - a^n b^m a^n : n,m >=0

ex 
S -> aSa| aBa
B -> bB | b                  by looking at bottom rules we can see that B makes b+ 
(a^n b^m a^n : n,m >=1)

ex
S -> SS|aS|b
- `a*b a*b` incorrect 
	- no bc 
	- S -> SS
	- S -> SSS
- `(a*b)^+`
	- in english: nonempty and ends with b
![[IMG_0101.jpg]]

- final ans: Σ* b

ex 
S-> AB
A->aAa|ε
B-> bBbε
- (bb)*
- (aa)*
- `(aa)*(bb)*` , n,m >= 0

ex 
S-> ε|aT|bT
T ->aS |bS

- (ΣΣ)*


